riscv crefine: setup proofs for clz and ctz
Progress towards verification of new and more efficient implementations
of library functions to could leading and trailing zeros.

Signed-off-by: Matthew Brecknell <Matthew.Brecknell@data61.csiro.au>

proof/crefine/RISCV64/Machine_C.thy
@@ -130,6 +130,155 @@ lemma dmo_if:
   "(doMachineOp (if a then b else c)) = (if a then (doMachineOp b) else (doMachineOp c))"
   by (simp split: if_split)
 
-end
+(* Count leading and trailing zeros. *)
 
+(* FIXME: move *)
+lemma word_ctz_max:
+  "word_ctz w \<le> size w"
+  sorry
+
+(* FIXME move *)
+lemma scast_of_nat_small:
+  "x < 2 ^ (LENGTH('a) - 1) \<Longrightarrow> scast (of_nat x :: 'a :: len word) = (of_nat x :: 'b :: len word)"
+  apply (rule sym, subst word_unat.inverse_norm)
+  apply (simp add: scast_def word_of_int[symmetric]
+                   of_nat_nat[symmetric] unat_def[symmetric])
+  apply (simp add: int_eq_sint unat_of_nat)
+  done
+
+(* FIXME move *)
+lemmas casts_of_nat_small = ucast_of_nat_small scast_of_nat_small
+
+(* FIXME: move *)
+lemma hoarep_Seq_nothrow:
+  assumes c: "hoarep \<Gamma> \<Theta> F P c Q {}"
+  assumes d: "hoarep \<Gamma> \<Theta> F Q d R A"
+  shows "hoarep \<Gamma> \<Theta> F P (Seq c d) R A"
+  by (rule hoarep.Seq[OF HoarePartialDef.conseqPrePost[OF c] d]; simp)
+
+definition clz32_step where
+  "clz32_step i \<equiv> \<acute>mask___unsigned :== \<acute>mask___unsigned >> unat ((1::32 sword) << unat i);;
+                 \<acute>bits :== SCAST(32 signed \<rightarrow> 32) (if \<acute>mask___unsigned < \<acute>x___unsigned then 1 else 0) << unat i;;
+                 Guard ShiftError \<lbrace>\<acute>bits < SCAST(32 signed \<rightarrow> 32) 0x20\<rbrace> (\<acute>x___unsigned :== \<acute>x___unsigned >> unat \<acute>bits);;
+                 \<acute>count :== \<acute>count - \<acute>bits"
+
+(* FIXME: figure out what this should be *)
+definition clz32_invariant where
+  "clz32_invariant i s \<equiv> {s'. undefined ''clz32_invariant'' i s s'}"
+
+lemma clz32_step:
+  "\<Gamma> \<turnstile> (clz32_invariant (i+1) s) clz32_step i (clz32_invariant i s)"
+  unfolding clz32_step_def
+  apply (vcg, clarsimp simp: clz32_invariant_def)
+  sorry
+
+lemma clz32_spec:
+  "\<forall>s. \<Gamma> \<turnstile> {s} Call clz32_'proc \<lbrace>\<acute>ret__unsigned = of_nat (word_clz (x___unsigned_' s))\<rbrace>"
+  apply (hoare_rule HoarePartial.ProcNoRec1)
+  apply (hoarep_rewrite, fold clz32_step_def)
+  apply (intro allI hoarep.Catch[OF _ hoarep.Skip])
+  apply (rule_tac Q="clz32_invariant 0 s" in hoarep_Seq_nothrow[OF _ creturn_wp])
+  apply (rule HoarePartial.SeqSwap[OF clz32_step], simp)+
+  apply (rule conseqPre, vcg)
+  apply (all \<open>clarsimp simp: clz32_invariant_def\<close>)
+  sorry
+
+definition clz64_step where
+  "clz64_step i \<equiv> \<acute>mask___unsigned_longlong :== \<acute>mask___unsigned_longlong >> unat ((1::32 sword) << unat i);;
+                   \<acute>bits :== SCAST(32 signed \<rightarrow> 32) (if \<acute>mask___unsigned_longlong < \<acute>x___unsigned_longlong then 1 else 0) << unat i;;
+                   Guard ShiftError \<lbrace>\<acute>bits < SCAST(32 signed \<rightarrow> 32) 0x40\<rbrace> (\<acute>x___unsigned_longlong :== \<acute>x___unsigned_longlong >> unat \<acute>bits);;
+                   \<acute>count :== \<acute>count - \<acute>bits"
+
+(* FIXME: figure out what this should be *)
+definition clz64_invariant where
+  "clz64_invariant i s \<equiv> {s'. undefined ''clz64_invariant'' i s s'}"
+
+lemma clz64_step:
+  "\<Gamma> \<turnstile> (clz64_invariant (i+1) s) clz64_step i (clz64_invariant i s)"
+  unfolding clz64_step_def
+  apply (vcg, clarsimp simp: clz64_invariant_def)
+  sorry
+
+lemma clz64_spec:
+  "\<forall>s. \<Gamma> \<turnstile> {s} Call clz64_'proc \<lbrace>\<acute>ret__unsigned = of_nat (word_clz (x___unsigned_longlong_' s))\<rbrace>"
+  apply (hoare_rule HoarePartial.ProcNoRec1)
+  apply (hoarep_rewrite, fold clz64_step_def)
+  apply (intro allI hoarep.Catch[OF _ hoarep.Skip])
+  apply (rule_tac Q="clz64_invariant 0 s" in hoarep_Seq_nothrow[OF _ creturn_wp])
+  apply (rule HoarePartial.SeqSwap[OF clz64_step], simp)+
+  apply (rule conseqPre, vcg)
+  apply (all \<open>clarsimp simp: clz64_invariant_def\<close>)
+  sorry
+
+definition ctz32_step where
+  "ctz32_step i \<equiv> \<acute>mask___unsigned :== \<acute>mask___unsigned >> unat ((1::32 sword) << unat i);;
+                   \<acute>bits :== SCAST(32 signed \<rightarrow> 32) (if \<acute>x___unsigned && \<acute>mask___unsigned = SCAST(32 signed \<rightarrow> 32) 0 then 1 else 0) << unat i;;
+                   Guard ShiftError \<lbrace>\<acute>bits < SCAST(32 signed \<rightarrow> 32) 0x20\<rbrace> (\<acute>x___unsigned :== \<acute>x___unsigned >> unat \<acute>bits);;
+                   \<acute>count :== \<acute>count + \<acute>bits"
+
+(* FIXME: figure out what this should be *)
+definition ctz32_invariant where
+  "ctz32_invariant i s \<equiv> {s'. undefined ''ctz32_invariant'' i s s'}"
+
+lemma ctz32_step:
+  "\<Gamma> \<turnstile> (ctz32_invariant (i+1) s) ctz32_step i (ctz32_invariant i s)"
+  unfolding ctz32_step_def
+  apply (vcg, clarsimp simp: ctz32_invariant_def)
+  sorry
+
+lemma ctz32_spec:
+  "\<forall>s. \<Gamma> \<turnstile> {s} Call ctz32_'proc \<lbrace>\<acute>ret__unsigned = of_nat (word_ctz (x___unsigned_' s))\<rbrace>"
+  apply (hoare_rule HoarePartial.ProcNoRec1)
+  apply (hoarep_rewrite, fold ctz32_step_def)
+  apply (intro allI hoarep.Catch[OF _ hoarep.Skip])
+  apply (rule_tac Q="ctz32_invariant 0 s" in hoarep_Seq_nothrow[OF _ creturn_wp])
+  apply (rule HoarePartial.SeqSwap[OF ctz32_step], simp)+
+  apply (rule conseqPre, vcg)
+  apply (all \<open>clarsimp simp: ctz32_invariant_def\<close>)
+  sorry
+
+definition ctz64_step where
+  "ctz64_step i \<equiv> \<acute>mask___unsigned_longlong :== \<acute>mask___unsigned_longlong >> unat ((1::32 sword) << unat i);;
+                   \<acute>bits :== SCAST(32 signed \<rightarrow> 32) (if \<acute>x___unsigned_longlong && \<acute>mask___unsigned_longlong = SCAST(32 signed \<rightarrow> 64) 0 then 1 else 0) << unat i;;
+                   Guard ShiftError \<lbrace>\<acute>bits < SCAST(32 signed \<rightarrow> 32) 0x40\<rbrace> (\<acute>x___unsigned_longlong :== \<acute>x___unsigned_longlong >> unat \<acute>bits);;
+                   \<acute>count :== \<acute>count + \<acute>bits"
+
+(* FIXME: figure out what this should be *)
+definition ctz64_invariant where
+  "ctz64_invariant i s \<equiv> {s'. undefined ''ctz64_invariant'' i s s'}"
+
+lemma ctz64_step:
+  "\<Gamma> \<turnstile> (ctz64_invariant (i+1) s) ctz64_step i (ctz64_invariant i s)"
+  unfolding ctz64_step_def
+  apply (vcg, clarsimp simp: ctz64_invariant_def)
+  sorry
+
+lemma ctz64_spec:
+  "\<forall>s. \<Gamma> \<turnstile> {s} Call ctz64_'proc \<lbrace>\<acute>ret__unsigned = of_nat (word_ctz (x___unsigned_longlong_' s))\<rbrace>"
+  apply (hoare_rule HoarePartial.ProcNoRec1)
+  apply (hoarep_rewrite, fold ctz64_step_def)
+  apply (intro allI hoarep.Catch[OF _ hoarep.Skip])
+  apply (rule_tac Q="ctz64_invariant 0 s" in hoarep_Seq_nothrow[OF _ creturn_wp])
+  apply (rule HoarePartial.SeqSwap[OF ctz64_step], simp)+
+  apply (rule conseqPre, vcg)
+  apply (all \<open>clarsimp simp: ctz64_invariant_def\<close>)
+  sorry
+
+(* The library implementations would allow us to weaken the preconditions to allow zero inputs,
+   but we keep the stronger preconditions to preserve older proofs that use these specs. *)
+lemma clzl_spec:
+  "\<forall>s. \<Gamma> \<turnstile> {\<sigma>. s = \<sigma> \<and> x___unsigned_long_' s \<noteq> 0}
+   Call clzl_'proc
+   \<lbrace>\<acute>ret__long = of_nat (word_clz (x___unsigned_long_' s))\<rbrace>"
+  apply (rule allI, rule conseqPre, vcg)
+  by (clarsimp simp: casts_of_nat_small[OF word_clz_max[THEN le_less_trans]] word_size)
+
+lemma ctzl_spec:
+  "\<forall>s. \<Gamma> \<turnstile> {\<sigma>. s = \<sigma> \<and> x___unsigned_long_' s \<noteq> 0}
+   Call ctzl_'proc
+   \<lbrace>\<acute>ret__long = of_nat (word_ctz (x___unsigned_long_' s))\<rbrace>"
+  apply (rule allI, rule conseqPre, vcg)
+  by (clarsimp simp: casts_of_nat_small[OF word_ctz_max[THEN le_less_trans]] word_size)
+
+end
 end
