proof/crefine/RISCV64/Syscall_C.thy
@@ -1595,16 +1595,6 @@ lemma ucast_maxIRQ_is_not_less:
   apply (erule notE)
   using ucast_up_mono by fastforce
 
-(* FIXME ARMHYP: move *)
-lemma ctzl_spec:
-  "\<forall>s. \<Gamma> \<turnstile> {\<sigma>. s = \<sigma> \<and> x_' s \<noteq> 0} Call ctzl_'proc
-       \<lbrace>\<acute>ret__long = of_nat (word_ctz (x_' s)) \<rbrace>"
-  apply (rule allI, rule conseqPre, vcg)
-  apply clarsimp
-  apply (rule_tac x="ret__long_'_update f x" for f in exI)
-  apply (simp add: mex_def meq_def)
-  done
-
 lemma ccorres_return_void_C_Seq:
   "ccorres_underlying sr \<Gamma> r rvxf arrel xf P P' hs X (return_void_C) \<Longrightarrow>
       ccorres_underlying sr \<Gamma> r rvxf arrel xf P P' hs X (return_void_C ;; Z)"
